rocq/runtime/wasm_api.ml
@@ -1,0 +1,13 @@
+open Js_of_ocaml
+
+let check_source source =
+  source |> Js.to_string |> String.to_seq |> List.of_seq
+  |> Report_json.checker_output |> Js.string
+
+let parse_presentation source =
+  source |> Js.to_string |> String.to_seq |> List.of_seq
+  |> Report_json.presentation_output |> Js.string
+
+let () =
+  Js.export "enderCheckProof" (Js.wrap_callback check_source);
+  Js.export "enderParsePresentation" (Js.wrap_callback parse_presentation)
