rocq/Ender/Extract.v
@@ -3,4 +3,5 @@ Require Import Ender.CertifiedAPI.
 
 Extraction Language OCaml.
 Extraction "extracted/EnderChecker.ml"
-  CertifiedAPI.parseProblem CertifiedAPI.check CertifiedAPI.checker.
+  CertifiedAPI.parseProblem CertifiedAPI.parsePresentation
+  CertifiedAPI.check CertifiedAPI.checker.
